add Customer class

LoanApplicationProcessing/User.dfy
@@ -1,12 +1,99 @@
 module {:extern "User"} User
 {
+  export provides Customer
   class Customer {
     // class constants
-    // class variables
+
+    // class variables  --------- not available in Dafny
+    
     // class methods
+    
     // instance constants
+
+    const	name: string 								
+    const	age: nat
+    const	accountNumber: string
+    const	sortCode: string
+    const	monthlyIncome: real
+    const	monthlyOutgoings: real
+    const referenceGenerator: Reference
+    
     // instance variables
+    var customerReference: nat
+
     // constructor
+    constructor(aName: string, anAge: nat, anAccountNumber: string, aSortCode: string, aMonthlyIncome: real, aMonthlyOutgoing: real)
+    ensures this.name == aName
+    ensures this.age == anAge
+    ensures this.accountNumber == anAccountNumber
+    ensures this.sortCode == aSortCode
+    ensures this.monthlyIncome == aMonthlyIncome
+    ensures this.monthlyOutgoings == aMonthlyOutgoing
+    {
+	    this.name := aName;
+	    this.age := anAge;
+	    this.accountNumber := anAccountNumber;
+	    this.sortCode := aSortCode;
+	    this.monthlyIncome := aMonthlyIncome;
+	    this.monthlyOutgoings := aMonthlyOutgoing;
+      this.referenceGenerator := new Reference();
+      new;
+      this.customerReference := this.referenceGenerator.getReferenceNumber();
+    }
+    
     // instance methods
+    method getName() returns (customerName: string)
+    ensures customerName == this.name
+    {
+	    return this.name;
+    }
+
+    method getAge() returns (customerAge: nat)
+    ensures customerAge == this.age
+    {
+      return this.age;  
+    }
+
+    method getPaymentDetails() returns (accountNumber: string, sortCode: string)
+    ensures accountNumber == this.accountNumber
+    ensures sortCode == this.sortCode
+    {
+      return this.accountNumber, this.sortCode;
+    }
+
+    method getMonthlyIncome() returns (income: real)
+    ensures income == this.monthlyIncome
+    {
+      return this.monthlyIncome;
+    }
+
+    method getMonthlyOutgoings() returns (outgoings: real)
+    ensures outgoings == this.monthlyOutgoings
+    {
+      return this.monthlyOutgoings;
+    }
+
+    method getCustomerReference() returns (reference: nat)
+    ensures reference == this.customerReference
+    {
+      return this.customerReference;
+    }
+  }
+
+  class Reference {
+    var reference: nat
+    constructor ()
+    {
+      reference := 1_000_000;
+    }
+    method getReferenceNumber() returns (ref: nat)
+    modifies this`reference
+    ensures ref == old(this.reference)
+    ensures this.reference == old(this.reference) + 1
+    {
+      var ref_old: nat := this.reference;
+      this.reference := this.reference + 1;
+      return ref_old;
+    }
   }
 }
